Almost complete core of acquire

ulib/experimental/Steel.SpinLock.fst
@@ -1,38 +1,80 @@
 module Steel.SpinLock
 open Steel.Effect
-//open Steel.Effect.Atomic
+open Steel.Effect.Atomic
 open Steel.Permissions
 open Steel.Reference
 open Steel.Actions
+open FStar.Ghost
 
 let available = false
 let locked = true
 
+unfold
 let lockinv (p:hprop) (r:ref bool) : hprop =
-  h_or (pts_to r full_permission available `star` p) (pts_to r full_permission locked)
+  h_or (pts_to r full_permission available `star` p) (pts_to r full_permission locked `star` emp)
 
 let lock (p:hprop) = (r:ref bool) & inv (lockinv p r)
-
-assume
-val new_inv (p:hprop) : SteelT (inv p) p (fun _ -> emp)
 
 assume
 val h_admit (#a:_) (p:hprop) (q:a -> hprop)
   : SteelT a p q
 
 assume
+val h_admit_atomic (#a:_) (#uses:Set.set lock_addr) (p:hprop) (q:a -> hprop)
+  : SteelAtomic a uses true p q
+
+
+assume
 val h_assert (p:hprop)
   : SteelT unit p (fun _ -> p)
+
+assume
+val h_assert_atomic (#uses:Set.set lock_addr) (p:hprop)
+  : SteelAtomic unit uses true p (fun _ -> p)
+
+assume
+val h_intro_emp_l (p:hprop)
+  : SteelAtomic unit Set.empty true p (fun _ -> emp `star` p)
+
+assume
+val h_commute (p q:hprop)
+  : SteelAtomic unit Set.empty true (p `star` q) (fun _ -> q `star` p)
+
 
 assume
 val intro_h_or_left (p:hprop) (q:hprop)
   : SteelT unit p (fun _ -> h_or p q)
 
+assume
+val intro_h_or_right (p:hprop) (q:hprop)
+  : SteelAtomic unit Set.empty true q (fun _ -> h_or p q)
+
 val intro_lockinv_left (p:hprop) (r:ref bool)
   : SteelT unit (pts_to r full_permission available `star` p) (fun _ -> lockinv p r)
 
+val intro_lockinv_right (p:hprop) (r:ref bool)
+  : SteelAtomic unit Set.empty true (pts_to r full_permission locked) (fun _ -> lockinv p r)
+
 let intro_lockinv_left p r =
-  intro_h_or_left (pts_to r full_permission available `star` p) (pts_to r full_permission locked)
+  intro_h_or_left
+    (pts_to r full_permission available `star` p)
+    (pts_to r full_permission locked `star` emp)
+
+let intro_lockinv_right p r =
+  h_intro_emp_l (pts_to r full_permission locked);
+  h_commute emp (pts_to r full_permission locked);
+  intro_h_or_right
+    (pts_to r full_permission available `star` p)
+    (pts_to r full_permission locked `star` emp)
+
+assume
+val lift_atomic_to_steelT
+  (#a:Type) (#is_ghost:bool) (#fp:hprop) (#fp':a -> hprop)
+  ($f:unit -> SteelAtomic a Set.empty is_ghost fp fp')
+  : SteelT a fp fp'
+
+val new_inv (p:hprop) : SteelT (inv p) p (fun _ -> emp)
+let new_inv p = lift_atomic_to_steelT (fun _ -> Steel.Effect.Atomic.new_inv p)
 
 let new_lock (p:hprop)
   : SteelT (lock p) p (fun _ -> emp) =
@@ -42,3 +84,80 @@ let new_lock (p:hprop)
   let i:inv (lockinv p r) = new_inv (lockinv p r) in
   let l:lock p = (| r, i |) in
   l
+
+/// A specialized version of get_ref_refine. It should be derivable from h_exists
+assume
+val ghost_read_or (#uses:Set.set lock_addr) (#p:perm) (r:ref bool)
+  (q:bool -> hprop)
+  : SteelAtomic bool uses true
+    (h_or (pts_to r p false `star` q false) (pts_to r p true `star` q true))
+    (fun x -> pts_to r p x `star` q x)
+
+assume
+val cas
+  (#t:eqtype)
+  (#uses:Set.set lock_addr)
+  (r:ref t)
+  (v:Ghost.erased t)
+  (v_old:t)
+  (v_new:t)
+  : SteelAtomic
+    (b:bool{b <==> (Ghost.reveal v == v_old)})
+    uses
+    false
+    (pts_to r full_permission v)
+    (fun b -> if b then pts_to r full_permission v_new else pts_to r full_permission v)
+
+assume
+val cas_frame
+  (#t:eqtype)
+  (#uses:Set.set lock_addr)
+  (r:ref t)
+  (v:Ghost.erased t)
+  (v_old:t)
+  (v_new:t)
+  (frame:hprop)
+  : SteelAtomic
+    (b:bool{b <==> (Ghost.reveal v == v_old)})
+    uses
+    false
+    (pts_to r full_permission v `star` frame)
+    (fun b -> (if b then pts_to r full_permission v_new else pts_to r full_permission v) `star` frame)
+
+
+assume
+val atomic_frame (#a:Type) (#pre:pre_t) (#post:post_t a)
+          (#uses:Set.set lock_addr) (#is_ghost:bool)
+          (frame:hprop)
+          ($f:unit -> SteelAtomic a uses is_ghost pre post)
+  : SteelAtomic a
+    uses is_ghost
+    (pre `star` frame)
+    (fun x -> post x `star` frame)
+
+val acquire_core (#p:hprop) (r:ref bool) (i:inv (lockinv p r))
+  : SteelAtomic bool Set.empty false
+    (lockinv p r)
+    (fun b -> lockinv p r `star` (if b then p else emp))
+
+let acquire_core #p r i =
+  let ghost = ghost_read_or r (fun b -> if b then emp else p) in
+  let frame = if ghost then emp else p in
+
+  let res = cas_frame r ghost available locked frame in
+
+  atomic_frame (if ghost then emp else p) (fun _ -> intro_lockinv_right p r);
+
+  h_assert_atomic (lockinv p r `star` (if res then p else emp));
+
+  h_admit_atomic
+    (lockinv p r `star` (if res then p else emp))
+    (fun b -> lockinv p r `star` (if b then p else emp))
+
+//TODO : Why is this failing? We have the postresource in the context
+//  res
+
+
+let acquire (#p:hprop) (l:lock p)
+  : SteelT unit emp (fun _ -> p)
+  = h_admit emp (fun _ -> p)
